a first version with a "univalent" universe

Cube.v
@@ -1,19 +1,35 @@
 Set Primitive Projections.
 Set Universe Polymorphism.
 
+Axiom proof_admitted : forall {a}, a.
+Tactic Notation "admit" := exact proof_admitted.
+
 Notation "x .1" := (projT1 x) (at level 3).
 Notation "x .2" := (projT2 x) (at level 3).
 Notation " ( x ; p ) " := (existT _ x p).
 
+(* CoInductive Glob : Type := *)
+(*   glob : forall Obj : Type, (Obj -> Obj -> Glob) -> Glob *)
+(* with *)
+(*  Elt : Type :=  *)
+(*   elt : forall (G:Glob) (here : match G with *)
+(*                  | glob Obj _ => Obj *)
+(*                  end), Elt (G.(eq) here here) -> Elt G. *)
+
 CoInductive Glob : Type :=
   { obj : Type ;
-    eq : forall x y : obj, Glob}.
+    eq : forall x y : obj, Glob
+  }.
 
 CoInductive elt (G:Glob): Type :=
   { here : G.(obj) ;
-    next : elt (G.(eq) here here)}.
+    next : elt (G.(eq) here here)  }.
 
-Definition Cubical : Type := { G : Glob & forall x, elt (G.(eq) x x)}. 
+CoInductive IsCubical (G:Glob) : Type :=
+  { refl : forall x, elt (G.(eq) x x);
+    eq_cubical : forall x y, IsCubical (G.(eq) x y)}.
+
+Definition Cubical : Type := { G : Glob & IsCubical G}.
 
 (* CoInductive hom (X Y : Glob) : Type := *)
 (*   { Gfun : X.(obj) -> Y.(obj); *)
@@ -22,19 +38,122 @@ Definition Cubical : Type := { G : Glob & forall x, elt (G.(eq) x x)}.
 (* Definition IsEqual X Y (f g : hom X Y) (x:X.(obj)) : Glob := *)
 (*     Y.(eq) (f.(Gfun _ _) x) (g.(Gfun _ _) x).  *)
 
-CoFixpoint _Typeᶠ : Glob := Build_Glob Glob (fun _ _ => _Typeᶠ).  
+CoFixpoint _Prodᶠ (A:Glob) (B : elt A -> Cubical) : Glob :=
+  Build_Glob (forall x: elt A, (B x).1.(obj))
+             (fun f g => _Prodᶠ A
+        (fun x => ((B x).1.(eq) (f x) (g x); (B x).2.(eq_cubical _) (f x) (g x)))).  
+
+Definition Prodᶠ_elt (A : Glob) : forall (Obj : elt A -> Type) (f : forall x : elt A, Obj x)
+     (F : forall x : elt A, Obj x -> Obj x -> Glob),
+   (forall (x : elt A) (e : Obj x), elt (F x e e)) ->
+   forall G : forall (x : elt A) (e e' : Obj x), IsCubical (F x e e'),
+     elt (_Prodᶠ A (fun x : elt A => (F x (f x) (f x); G x (f x) (f x)))).
+  cofix. intros Obj f F G' G. simple refine (Build_elt _ _ _).
+  + cbn. intro x. exact (G' _ _).(here _).
+  + cbn.
+    pose (_Obj := fun x => obj (F x (f x) (f x))).
+    pose (_f := fun x => (here (F x (f x) (f x)) (G' x (f x))): _Obj x).
+    pose (_F := fun x => eq (F x (f x) (f x))).
+    pose (_G := fun x => eq_cubical (F x (f x) (f x)) (G x (f x) (f x))).
+    pose (_G' := fun x => refl (F x (f x) (f x)) (G x (f x) (f x))).
+    refine (Prodᶠ_elt _Obj _f _F _G' _G).
+Defined. 
+
+CoFixpoint Prodᶠ_cubical (A:Glob) (B : elt A -> Cubical) : IsCubical (_Prodᶠ A B).
+econstructor.
+- intro f. cbn in *. 
+  set (Obj := fun x : elt A => obj (B x) .1).
+  change (forall x : elt A, Obj x) in f. 
+  set (F := fun x : elt A => eq (B x) .1 : Obj x -> Obj x -> Glob).
+  set (G := fun x : elt A => eq_cubical (B x) .1 (B x) .2 : forall e e', IsCubical (F x e e')).
+  set (G' := fun x : elt A => (B x).2.(refl _) : forall (e:Obj x), elt (F x e e)).
+  refine (Prodᶠ_elt _ Obj f F G' G).
+- intros f g. refine (Prodᶠ_cubical _ _).
+Defined.
+
+Definition Prodᶠ (A:Glob) (B : elt A -> Cubical) : Cubical :=
+  (_Prodᶠ A B; Prodᶠ_cubical A B).
+
+
+Record TypeEquiv (A B : Glob) : Type :=
+  {
+    equiv : A.(obj) -> B.(obj) ;
+    equiv_inv : B.(obj) -> A.(obj) ;
+    sect : forall x, (A.(eq) (equiv_inv (equiv x)) x).(obj);
+    retr : forall x, (B.(eq) (equiv (equiv_inv x)) x).(obj);
+    (* no adjunction required ? *)
+  }.
+
+Definition Equiv (A B : Cubical) : Cubical.
+Proof.
+  simple refine (existT _ _ _). 
+  - refine (Build_Glob (TypeEquiv A.1 B.1) (fun f g => _)).
+    exact (_Prodᶠ A.1 (fun x => (B.1.(eq) (f.(equiv _ _) x.(here _)) (g.(equiv _ _) x.(here _)); B.2.(eq_cubical _) _ _))).
+  - cbn. refine (Build_IsCubical _ _ _).
+    {
+    cbn. intro e. simple refine (Build_elt _ _ _).
+    + cbn. intro x. exact (B.2.(refl _) _).(here _).
+    + exact ((Prodᶠ_cubical A.1 (fun x : elt A .1 =>
+         (eq B .1 (equiv A .1 B .1 e (here A .1 x))
+            (equiv A .1 B .1 e (here A .1 x));
+         eq_cubical B .1 B .2 (equiv A .1 B .1 e (here A .1 x))
+                    (equiv A .1 B .1 e (here A .1 x))))).(refl _) _).
+    }
+    {
+      cbn. intros e e'.  exact (Prodᶠ_cubical _ _).
+    }
+Defined.
+
+Definition _Typeᶠ : Glob := Build_Glob Cubical (fun A B => (Equiv A B).1).  
+
+Definition Identity (A:Cubical) : TypeEquiv A.1 A.1.
+simple refine (Build_TypeEquiv _ _ (fun x => x) (fun x => x) _ _).
+- intros. exact ((A.2.(refl _) x).(here _)).
+- intros. exact ((A.2.(refl _) x).(here _)).
+Defined. 
+  
+(*
+Definition ID_eq (A:Cubical) : elt
+     (_Prodᶠ A .1 (fun x : elt A .1 => eq A .1 (here A .1 x) (here A .1 x))).
+Proof.
+  cbn in *. revert A. cofix. intro A. simple refine (Build_elt _ _ _).
+    + cbn. intros x. exact (x.(next _).(here _)).
+    + cbn. simple refine (Build_elt _ _ _).
+      * cbn. intro x. exact (x.(next _).(next _).(here _)).
+      * cbn. admit. 
+Admitted. 
+*)
 
 Definition Typeᶠ : Cubical.
 Proof.
   refine (existT _ _Typeᶠ _).
-  intros x. cofix. refine (Build_elt _Typeᶠ x Typeᶠ).
+  econstructor.
+  { intros A. simpl. simple refine (Build_elt _ _ _).
+    - simpl. exact (Identity A).
+    - cbn.
+      simple refine (Build_elt _ _ _).
+    + cbn. intro x. exact (A.2.(refl _) _).(here _).
+    + exact ((Prodᶠ_cubical A.1 _).(refl _) _).
+    }
+  {
+    intros X Y. cbn.  econstructor.
+    - cbn. intro e.
+      pose (Obj := fun x:elt X.1 => obj Y.1).
+      pose (f := fun x => (equiv X .1 Y .1 e (here X .1 x)) : Obj x).
+      pose (F := fun x : elt X .1 => eq Y .1).
+      pose (G' := fun x : elt X .1 => eq_cubical Y .1 Y .2).
+      pose (G := fun x : elt X .1 => refl Y .1 Y .2).
+      refine (Prodᶠ_elt X.1 Obj f F G G'). 
+    - intros e e'. cbn. exact (Prodᶠ_cubical X.1 _). 
+  }
 Defined. 
 
-CoFixpoint Prodᶠ (A:Glob) (B : elt A -> Typeᶠ.1.(obj)) : Glob :=
-  Build_Glob (forall x: elt A, (B x).(obj))
-             (fun f g => Prodᶠ A (fun x => (B x).(eq) (f x) (g x))).  
+CoFixpoint Prodᶠ (A:Cubical) (B : elt A.1 -> Typeᶠ.1.(obj)) : Glob.
+refine (  Build_Glob (forall x: elt A.1, (B x).1.(obj))
+             (fun f g => Prodᶠ A (fun x => ((B x).1.(eq) (f x) (g x) ; _)))).
+intros e. pose (  eq (B x) .1 (f x) (g x)). exact ((B x).2 (f x)).
 
-CoFixpoint Lamᶠ (A:Glob) (B : elt A -> Typeᶠ.1.(obj)) (t: forall x: elt A, elt (B x)) :
+CoFixpoint Lamᶠ (A:Glob) (B : elt A -> Typeᶠ.1.(obj)) (t: forall x: elt A, elt (B x).1) :
   elt (Prodᶠ A B).
 refine (Build_elt (Prodᶠ A B) (fun x => (t x).(here _)) _).
 cbn. apply Lamᶠ. intros x. apply ((t x).(next _)).
